Relational interpretation of strategy trees for (ErrorT (State S)).

Strategy.v
@@ -57,7 +57,7 @@ Lemma evaltree_same (t : Tree) (f : A -> B) :
   evaltree t f = evaltree_unit t f.
 Proof. induction t; now firstorder. Qed.
 
-(* Interpreter of trees for relations *)
+(* Relational interpreter of trees for (State S) *)
 Inductive wrap_rel_State {S}
   : Tree -> (A -> S -> B * S -> Prop) -> S -> C * S -> Prop :=
   | wrapAns :
@@ -102,6 +102,94 @@ induction t as [c | a k IH].
   now firstorder.
 Qed.
 
+(* Relational interpreter of trees for (ErrorT (State S)) *)
+Inductive wrap_rel_ErrorT_State {S}
+  : Tree -> (A -> S -> (Exc B) * S -> Prop) -> S -> (Exc C) * S -> Prop :=
+  | wrapESAns :
+      forall (f : A -> S -> (Exc B) * S -> Prop) c s,
+        wrap_rel_ErrorT_State (Ans c) f s (value c,s)
+  | wrapESQueValue :
+      forall (f : A -> S -> (Exc B) * S -> Prop) a k s d0 s0 ds1,
+        f a s (value d0, s0) ->
+        wrap_rel_ErrorT_State (k d0) f s0 ds1 ->
+        wrap_rel_ErrorT_State (Que a k) f s ds1
+  | wrapESQueError :
+      forall (f : A -> S -> (Exc B) * S -> Prop) a k s s0,
+        f a s (error, s0) ->
+        wrap_rel_ErrorT_State (Que a k) f s (error,s0).
+
+Lemma wrap_rel_ErrorT_State_Ans_inv S c f s d1 s1 :
+  @wrap_rel_ErrorT_State S (Ans c) f s (d1, s1) ->
+  d1 = value c /\ s1 = s.
+Proof. intros H; now inversion H; subst. Qed.
+
+Lemma wrap_rel_ErrorT_State_Que_value_inv S a k f s d s1 :
+  @wrap_rel_ErrorT_State S (Que a k) f s (value d,s1) ->
+  exists d0 s0,
+    f a s (value d0, s0) /\
+    wrap_rel_ErrorT_State (k d0) f s0 (value d,s1).
+Proof. intros H; now inversion H; subst; eauto. Qed.
+
+Lemma wrap_rel_ErrorT_State_Que_error_inv S a k f s s1 :
+  @wrap_rel_ErrorT_State S (Que a k) f s (error,s1) ->
+  f a s (error,s1) \/
+  exists d0 s0,
+    f a s (value d0, s0) /\
+    wrap_rel_ErrorT_State (k d0) f s0 (error,s1).
+Proof. intros H; now inversion H; subst; eauto. Qed.
+
+Lemma wrap_rel_ErrorT_State_fun S t
+  (f : A -> S -> (Exc B) * S -> Prop)
+  (f' : A -> S -> (Exc B) * S -> Prop)
+  (Hfun : forall a s r r', f a s r -> f' a s r' -> r = r') :
+  forall s ds1 ds1',
+    @wrap_rel_ErrorT_State S t f s ds1 ->
+    @wrap_rel_ErrorT_State S t f' s ds1' ->
+    ds1 = ds1'.
+Proof.
+induction t as [c | a k IH].
+- intros s [d1 s1] [d1' s1'] H H'.
+  destruct (wrap_rel_ErrorT_State_Ans_inv H); subst.
+  destruct (wrap_rel_ErrorT_State_Ans_inv H'); subst.
+  easy.
+- intros s [d1 s1] [d1' s1'] H H'.
+  destruct d1 as [d1 |]; destruct d1' as [d1' |].
+  + destruct (wrap_rel_ErrorT_State_Que_value_inv H)
+             as [d0 [s0 [Hf H0]]].
+    destruct (wrap_rel_ErrorT_State_Que_value_inv H')
+             as [d0' [s0' [Hf' H0']]].
+    assert (H1 := Hfun _ _ _ _ Hf Hf').
+    inversion H1; subst; clear H1.
+    now firstorder.
+  + destruct (wrap_rel_ErrorT_State_Que_value_inv H)
+             as [d0 [s0 [Hf H0]]].
+    destruct (wrap_rel_ErrorT_State_Que_error_inv H')
+             as [Hf' | [d0' [s0' [Hf' H0']]]].
+    * now assert (H1 := Hfun _ _ _ _ Hf Hf').
+    * assert (H1 := Hfun _ _ _ _ Hf Hf').
+      inversion H1; subst; clear H1.
+      now firstorder.
+  + destruct (wrap_rel_ErrorT_State_Que_value_inv H')
+             as [d0' [s0' [Hf' H0']]].
+    destruct (wrap_rel_ErrorT_State_Que_error_inv H)
+             as [Hf | [d0 [s0 [Hf H0]]]].
+    * now assert (H1 := Hfun _ _ _ _ Hf Hf').
+    * assert (H1 := Hfun _ _ _ _ Hf Hf').
+      inversion H1; subst; clear H1.
+      now firstorder.
+  + destruct (wrap_rel_ErrorT_State_Que_error_inv H)
+             as [Hf | [d0 [s0 [Hf H0]]]];
+    destruct (wrap_rel_ErrorT_State_Que_error_inv H')
+             as [Hf' | [d0' [s0' [Hf' H0']]]].
+    * assert (H1 := Hfun _ _ _ _ Hf Hf').
+      now inversion H1; subst; clear H1.
+    * now assert (H1 := Hfun _ _ _ _ Hf Hf').
+    * now assert (H1 := Hfun _ _ _ _ Hf Hf').
+    * assert (H1 := Hfun _ _ _ _ Hf Hf').
+      inversion H1; subst; clear H1.
+      now firstorder.
+Qed.
+
 End strategy.
 
 Implicit Arguments Ans [A B C].
@@ -110,6 +198,8 @@ Implicit Arguments Que [A B C].
 Notation "[[ t ]]" := (@tree2fun _ _ _ (t : Tree _ _ _)) (at level 60).
 Notation "[[ t ]]*" := (@evaltree _ _ _ (t : Tree _ _ _)) (at level 60).
 Notation "[[ t ]]#" := (@wrap_rel_State _ _ _ _ (t : Tree _ _ _)) (at level 60).
+Notation "[[ t ]]##" := (@wrap_rel_ErrorT_State _ _ _ _ (t : Tree _ _ _)) (at level 60).
+
 
 (*Definition isPure A B C (F : FuncType A B C)
   := exists t, forall (T : monadType), F T = [[t]] T.*)
